Update the tutorial

tests/src/tutorial/src/lib.rs
@@ -1,5 +1,152 @@
 pub type Bignum = Vec<u32>;
 
+pub fn choose<'a, T>(b: bool, x: &'a mut T, y: &'a mut T) -> &'a mut T {
+    if b {
+        x
+    } else {
+        y
+    }
+}
+
+pub fn mul2_add1(x: u32) -> u32 {
+    (x + x) + 1
+}
+
+pub fn mul2_add1_add(x: u32, y: u32) -> u32 {
+    mul2_add1(x) + y
+}
+
+pub fn incr<'a>(x: &'a mut u32) {
+    *x += 1;
+}
+
+pub fn use_incr() {
+    let mut x = 0;
+    incr(&mut x);
+    incr(&mut x);
+    incr(&mut x);
+}
+
+/* Recursion, loops */
+
+pub enum CList<T> {
+    CCons(T, Box<CList<T>>),
+    CNil,
+}
+
+pub fn list_nth<'a, T>(l: &'a CList<T>, i: u32) -> &'a T {
+    match l {
+        CList::CCons(x, tl) => {
+            if i == 0 {
+                x
+            } else {
+                list_nth(tl, i - 1)
+            }
+        }
+        CList::CNil => {
+            panic!()
+        }
+    }
+}
+
+pub fn list_nth_mut<'a, T>(l: &'a mut CList<T>, i: u32) -> &'a mut T {
+    match l {
+        CList::CCons(x, tl) => {
+            if i == 0 {
+                x
+            } else {
+                list_nth_mut(tl, i - 1)
+            }
+        }
+        CList::CNil => {
+            panic!()
+        }
+    }
+}
+
+pub fn list_nth1<'a, T>(mut l: &'a CList<T>, mut i: u32) -> &'a T {
+    while let CList::CCons(x, tl) = l {
+        if i == 0 {
+            return x;
+        }
+        i -= 1;
+        l = tl;
+    }
+    panic!()
+}
+
+pub fn i32_id(i : i32) -> i32 {
+    if i == 0 {
+        0
+    }
+    else {
+        i32_id(i - 1) + 1
+    }
+}
+
+pub fn even(i : u32) -> bool {
+    if i == 0 {
+        true
+    }
+    else {
+        odd(i - 1)
+    }
+}
+
+pub fn odd(i : u32) -> bool {
+    if i == 0 {
+        false
+    }
+    else {
+        even(i - 1)
+    }
+}
+
+/* Traits */
+
+pub trait Counter {
+    fn incr(&mut self) -> usize;
+}
+
+impl Counter for usize {
+    fn incr(&mut self) -> usize {
+        let x = *self;
+        *self += 1;
+        x
+    }
+}
+
+pub fn use_counter<'a, T: Counter>(cnt: &'a mut T) -> usize {
+    cnt.incr()
+}
+
+/* Exercises: warm up */
+
+pub fn list_nth_mut1<'a, T>(mut l: &'a mut CList<T>, mut i: u32) -> &'a mut T {
+    while let CList::CCons(x, tl) = l {
+        if i == 0 {
+            return x;
+        }
+        i -= 1;
+        l = tl;
+    }
+    panic!()
+}
+
+pub fn list_tail<'a, T>(mut l: &'a mut CList<T>) -> &'a mut CList<T> {
+    while let CList::CCons(_, tl) = l {
+        l = tl;
+    }
+    l
+}
+
+pub fn append_in_place<'a, T>(l0: &'a mut CList<T>,  l1 : CList<T>) {
+    let tl = list_tail(l0);
+    *tl = l1;
+}
+
+/* Big numbers */
+
 /// Zero out a bignum
 pub fn zero(x : &mut Bignum) {
     let mut i = 0;
@@ -22,7 +169,7 @@ pub fn add_no_overflow(x: &mut Bignum, y: &Bignum) {
     }
 }
 
-fn max(x : usize, y : usize) -> usize {
+fn usize_max(x : usize, y : usize) -> usize {
     if x > y { x } else { y }
 }
 
@@ -51,8 +198,10 @@ pub fn add_with_carry(x: &mut Bignum, y: &Bignum) -> u8 {
 /// Add a bignum in place.
 ///
 /// The bignums may have different lengths, and we resize x if necessary.
+/// Note: this is not what we usually do in cryptographic code, where big
+/// numbers have a fixed size, but is interesting as an exercise.
 pub fn add(x: &mut Bignum, y: &Bignum) {
-    let max = max(x.len(), y.len());
+    let max = usize_max(x.len(), y.len());
     x.resize(max, 0u32);
     // now: length x >= length y
     let mut c0 = 0u8;
