tests/lean/Tutorial/Tutorial.lean
@@ -8,8 +8,229 @@ set_option linter.unusedVariables false
 
 namespace tutorial
 
+/- [tutorial::choose]:
+   Source: 'src/lib.rs', lines 3:0-3:70 -/
+def choose
+  (T : Type) (b : Bool) (x : T) (y : T) :
+  Result (T × (T → Result (T × T)))
+  :=
+  if b
+  then let back := fun ret => Result.ok (ret, y)
+       Result.ok (x, back)
+  else let back := fun ret => Result.ok (x, ret)
+       Result.ok (y, back)
+
+/- [tutorial::mul2_add1]:
+   Source: 'src/lib.rs', lines 11:0-11:31 -/
+def mul2_add1 (x : U32) : Result U32 :=
+  do
+  let i ← x + x
+  i + 1#u32
+
+/- [tutorial::mul2_add1_add]:
+   Source: 'src/lib.rs', lines 15:0-15:43 -/
+def mul2_add1_add (x : U32) (y : U32) : Result U32 :=
+  do
+  let i ← mul2_add1 x
+  i + y
+
+/- [tutorial::incr]:
+   Source: 'src/lib.rs', lines 19:0-19:31 -/
+def incr (x : U32) : Result U32 :=
+  x + 1#u32
+
+/- [tutorial::use_incr]:
+   Source: 'src/lib.rs', lines 23:0-23:17 -/
+def use_incr : Result Unit :=
+  do
+  let x ← incr 0#u32
+  let x1 ← incr x
+  let _ ← incr x1
+  Result.ok ()
+
+/- [tutorial::CList]
+   Source: 'src/lib.rs', lines 32:0-32:17 -/
+inductive CList (T : Type) :=
+| CCons : T → CList T → CList T
+| CNil : CList T
+
+/- [tutorial::list_nth]:
+   Source: 'src/lib.rs', lines 37:0-37:56 -/
+divergent def list_nth (T : Type) (l : CList T) (i : U32) : Result T :=
+  match l with
+  | CList.CCons x tl =>
+    if i = 0#u32
+    then Result.ok x
+    else do
+         let i1 ← i - 1#u32
+         list_nth T tl i1
+  | CList.CNil => Result.fail .panic
+
+/- [tutorial::list_nth_mut]:
+   Source: 'src/lib.rs', lines 52:0-52:68 -/
+divergent def list_nth_mut
+  (T : Type) (l : CList T) (i : U32) :
+  Result (T × (T → Result (CList T)))
+  :=
+  match l with
+  | CList.CCons x tl =>
+    if i = 0#u32
+    then
+      let back := fun ret => Result.ok (CList.CCons ret tl)
+      Result.ok (x, back)
+    else
+      do
+      let i1 ← i - 1#u32
+      let (t, list_nth_mut_back) ← list_nth_mut T tl i1
+      let back :=
+        fun ret =>
+          do
+          let tl1 ← list_nth_mut_back ret
+          Result.ok (CList.CCons x tl1)
+      Result.ok (t, back)
+  | CList.CNil => Result.fail .panic
+
+/- [tutorial::list_nth1]: loop 0:
+   Source: 'src/lib.rs', lines 67:0-76:1 -/
+divergent def list_nth1_loop (T : Type) (l : CList T) (i : U32) : Result T :=
+  match l with
+  | CList.CCons x tl =>
+    if i = 0#u32
+    then Result.ok x
+    else do
+         let i1 ← i - 1#u32
+         list_nth1_loop T tl i1
+  | CList.CNil => Result.fail .panic
+
+/- [tutorial::list_nth1]:
+   Source: 'src/lib.rs', lines 67:0-67:65 -/
+@[reducible]
+def list_nth1 (T : Type) (l : CList T) (i : U32) : Result T :=
+  list_nth1_loop T l i
+
+/- [tutorial::i32_id]:
+   Source: 'src/lib.rs', lines 78:0-78:29 -/
+divergent def i32_id (i : I32) : Result I32 :=
+  if i = 0#i32
+  then Result.ok 0#i32
+  else do
+       let i1 ← i - 1#i32
+       let i2 ← i32_id i1
+       i2 + 1#i32
+
+/- [tutorial::even]:
+   Source: 'src/lib.rs', lines 87:0-87:28 -/
+mutual divergent def even (i : U32) : Result Bool :=
+  if i = 0#u32
+  then Result.ok true
+  else do
+       let i1 ← i - 1#u32
+       odd i1
+
+/- [tutorial::odd]:
+   Source: 'src/lib.rs', lines 96:0-96:27 -/
+divergent def odd (i : U32) : Result Bool :=
+  if i = 0#u32
+  then Result.ok false
+  else do
+       let i1 ← i - 1#u32
+       even i1
+
+end
+
+/- Trait declaration: [tutorial::Counter]
+   Source: 'src/lib.rs', lines 107:0-107:17 -/
+structure Counter (Self : Type) where
+  incr : Self → Result (Usize × Self)
+
+/- [tutorial::{tutorial::Counter for usize}::incr]:
+   Source: 'src/lib.rs', lines 112:4-112:31 -/
+def CounterUsize.incr (self : Usize) : Result (Usize × Usize) :=
+  do
+  let self1 ← self + 1#usize
+  Result.ok (self, self1)
+
+/- Trait implementation: [tutorial::{tutorial::Counter for usize}]
+   Source: 'src/lib.rs', lines 111:0-111:22 -/
+@[reducible]
+def CounterUsize : Counter Usize := {
+  incr := CounterUsize.incr
+}
+
+/- [tutorial::use_counter]:
+   Source: 'src/lib.rs', lines 119:0-119:59 -/
+def use_counter
+  (T : Type) (CounterInst : Counter T) (cnt : T) : Result (Usize × T) :=
+  CounterInst.incr cnt
+
+/- [tutorial::list_nth_mut1]: loop 0:
+   Source: 'src/lib.rs', lines 125:0-134:1 -/
+divergent def list_nth_mut1_loop
+  (T : Type) (l : CList T) (i : U32) :
+  Result (T × (T → Result (CList T)))
+  :=
+  match l with
+  | CList.CCons x tl =>
+    if i = 0#u32
+    then
+      let back := fun ret => Result.ok (CList.CCons ret tl)
+      Result.ok (x, back)
+    else
+      do
+      let i1 ← i - 1#u32
+      let (t, back) ← list_nth_mut1_loop T tl i1
+      let back1 :=
+        fun ret => do
+                   let tl1 ← back ret
+                   Result.ok (CList.CCons x tl1)
+      Result.ok (t, back1)
+  | CList.CNil => Result.fail .panic
+
+/- [tutorial::list_nth_mut1]:
+   Source: 'src/lib.rs', lines 125:0-125:77 -/
+@[reducible]
+def list_nth_mut1
+  (T : Type) (l : CList T) (i : U32) :
+  Result (T × (T → Result (CList T)))
+  :=
+  list_nth_mut1_loop T l i
+
+/- [tutorial::list_tail]: loop 0:
+   Source: 'src/lib.rs', lines 136:0-141:1 -/
+divergent def list_tail_loop
+  (T : Type) (l : CList T) :
+  Result ((CList T) × (CList T → Result (CList T)))
+  :=
+  match l with
+  | CList.CCons t tl =>
+    do
+    let (c, back) ← list_tail_loop T tl
+    let back1 :=
+      fun ret => do
+                 let tl1 ← back ret
+                 Result.ok (CList.CCons t tl1)
+    Result.ok (c, back1)
+  | CList.CNil => Result.ok (CList.CNil, Result.ok)
+
+/- [tutorial::list_tail]:
+   Source: 'src/lib.rs', lines 136:0-136:68 -/
+@[reducible]
+def list_tail
+  (T : Type) (l : CList T) :
+  Result ((CList T) × (CList T → Result (CList T)))
+  :=
+  list_tail_loop T l
+
+/- [tutorial::append_in_place]:
+   Source: 'src/lib.rs', lines 143:0-143:67 -/
+def append_in_place
+  (T : Type) (l0 : CList T) (l1 : CList T) : Result (CList T) :=
+  do
+  let (_, list_tail_back) ← list_tail T l0
+  list_tail_back l1
+
 /- [tutorial::zero]: loop 0:
-   Source: 'src/lib.rs', lines 5:4-10:1 -/
+   Source: 'src/lib.rs', lines 152:4-157:1 -/
 divergent def zero_loop
   (x : alloc.vec.Vec U32) (i : Usize) : Result (alloc.vec.Vec U32) :=
   let i1 := alloc.vec.Vec.len U32 x
@@ -25,12 +246,12 @@ divergent def zero_loop
   else Result.ok x
 
 /- [tutorial::zero]:
-   Source: 'src/lib.rs', lines 4:0-4:28 -/
+   Source: 'src/lib.rs', lines 151:0-151:28 -/
 def zero (x : alloc.vec.Vec U32) : Result (alloc.vec.Vec U32) :=
   zero_loop x 0#usize
 
 /- [tutorial::add_no_overflow]: loop 0:
-   Source: 'src/lib.rs', lines 18:4-23:1 -/
+   Source: 'src/lib.rs', lines 165:4-170:1 -/
 divergent def add_no_overflow_loop
   (x : alloc.vec.Vec U32) (y : alloc.vec.Vec U32) (i : Usize) :
   Result (alloc.vec.Vec U32)
@@ -52,22 +273,22 @@ divergent def add_no_overflow_loop
   else Result.ok x
 
 /- [tutorial::add_no_overflow]:
-   Source: 'src/lib.rs', lines 17:0-17:50 -/
+   Source: 'src/lib.rs', lines 164:0-164:50 -/
 def add_no_overflow
   (x : alloc.vec.Vec U32) (y : alloc.vec.Vec U32) :
   Result (alloc.vec.Vec U32)
   :=
   add_no_overflow_loop x y 0#usize
 
-/- [tutorial::max]:
-   Source: 'src/lib.rs', lines 25:0-25:37 -/
-def max (x : Usize) (y : Usize) : Result Usize :=
+/- [tutorial::usize_max]:
+   Source: 'src/lib.rs', lines 172:0-172:43 -/
+def usize_max (x : Usize) (y : Usize) : Result Usize :=
   if x > y
   then Result.ok x
   else Result.ok y
 
 /- [tutorial::get_or_zero]:
-   Source: 'src/lib.rs', lines 29:0-29:45 -/
+   Source: 'src/lib.rs', lines 176:0-176:45 -/
 def get_or_zero (y : alloc.vec.Vec U32) (i : Usize) : Result U32 :=
   let i1 := alloc.vec.Vec.len U32 y
   if i < i1
@@ -77,7 +298,7 @@ def get_or_zero (y : alloc.vec.Vec U32) (i : Usize) : Result U32 :=
   else Result.ok 0#u32
 
 /- [tutorial::add_with_carry]: loop 0:
-   Source: 'src/lib.rs', lines 38:4-49:1 -/
+   Source: 'src/lib.rs', lines 185:4-196:1 -/
 divergent def add_with_carry_loop
   (x : alloc.vec.Vec U32) (y : alloc.vec.Vec U32) (c0 : U8) (i : Usize) :
   Result (U8 × (alloc.vec.Vec U32))
@@ -109,7 +330,7 @@ divergent def add_with_carry_loop
   else Result.ok (c0, x)
 
 /- [tutorial::add_with_carry]:
-   Source: 'src/lib.rs', lines 36:0-36:55 -/
+   Source: 'src/lib.rs', lines 183:0-183:55 -/
 def add_with_carry
   (x : alloc.vec.Vec U32) (y : alloc.vec.Vec U32) :
   Result (U8 × (alloc.vec.Vec U32))
@@ -117,13 +338,13 @@ def add_with_carry
   add_with_carry_loop x y 0#u8 0#usize
 
 /- [tutorial::add]: loop 0:
-   Source: 'src/lib.rs', lines 59:4-75:1 -/
+   Source: 'src/lib.rs', lines 208:4-224:1 -/
 divergent def add_loop
-  (x : alloc.vec.Vec U32) (y : alloc.vec.Vec U32) (max1 : Usize) (c0 : U8)
+  (x : alloc.vec.Vec U32) (y : alloc.vec.Vec U32) (max : Usize) (c0 : U8)
   (i : Usize) :
   Result (alloc.vec.Vec U32)
   :=
-  if i < max1
+  if i < max
   then
     do
     let yi ← get_or_zero y i
@@ -143,7 +364,7 @@ divergent def add_loop
         (core.slice.index.SliceIndexUsizeSliceTInst U32) x i
     let i5 ← i + 1#usize
     let x1 ← index_mut_back sum1
-    add_loop x1 y max1 c01 i5
+    add_loop x1 y max c01 i5
   else
     if c0 != 0#u8
     then do
@@ -152,7 +373,7 @@ divergent def add_loop
     else Result.ok x
 
 /- [tutorial::add]:
-   Source: 'src/lib.rs', lines 54:0-54:38 -/
+   Source: 'src/lib.rs', lines 203:0-203:38 -/
 def add
   (x : alloc.vec.Vec U32) (y : alloc.vec.Vec U32) :
   Result (alloc.vec.Vec U32)
@@ -160,8 +381,8 @@ def add
   do
   let i := alloc.vec.Vec.len U32 x
   let i1 := alloc.vec.Vec.len U32 y
-  let max1 ← max i i1
-  let x1 ← alloc.vec.Vec.resize U32 core.clone.CloneU32 x max1 0#u32
-  add_loop x1 y max1 0#u8 0#usize
+  let max ← usize_max i i1
+  let x1 ← alloc.vec.Vec.resize U32 core.clone.CloneU32 x max 0#u32
+  add_loop x1 y max 0#u8 0#usize
 
 end tutorial
